ArkLib.lean
@@ -280,10 +280,7 @@ import ArkLib.Data.Probability.Notation
 import ArkLib.Interaction.Oracle.Protocol
 import ArkLib.Interaction.Oracle.TypeTree
 import ArkLib.Interaction.Oracle.TypeTree.Decoration
-import ArkLib.Interaction.Oracle.TypeTree.DecorationExample
-import ArkLib.Interaction.Oracle.TypeTree.MixedExample
 import ArkLib.Interaction.Reduction
-import ArkLib.Interaction.Reduction.DependentExample
 import ArkLib.OracleReduction.BCS.Basic
 import ArkLib.OracleReduction.Basic
 import ArkLib.OracleReduction.Cast
